examples/ghc/lib/Maybes.v
@@ -40,14 +40,17 @@ Local Definition Functor__MaybeErr_fmap {inst_err}
       | Failed e => Failed e
       end.
 
-Local Definition Functor__MaybeErr_op_zlzd__ {inst_err}
-   : forall {a} {b}, a -> (MaybeErr inst_err) b -> (MaybeErr inst_err) a :=
-  fun {a} {b} => Functor__MaybeErr_fmap GHC.Base.∘ GHC.Base.const.
+Local Definition Functor__MaybeErr_op_zlzd__ {inst_err : Type}
+   : forall {a : Type},
+     forall {b : Type}, a -> MaybeErr inst_err b -> MaybeErr inst_err a :=
+  fun {a : Type} {b : Type} => Functor__MaybeErr_fmap GHC.Base.∘ GHC.Base.const.
 
-Program Instance Functor__MaybeErr {err} : GHC.Base.Functor (MaybeErr err) :=
+Program Instance Functor__MaybeErr {err : Type}
+   : GHC.Base.Functor (MaybeErr err) :=
   fun _ k__ =>
-    k__ {| GHC.Base.fmap__ := fun {a} {b} => Functor__MaybeErr_fmap ;
-           GHC.Base.op_zlzd____ := fun {a} {b} => Functor__MaybeErr_op_zlzd__ |}.
+    k__ {| GHC.Base.fmap__ := fun {a : Type} {b : Type} => Functor__MaybeErr_fmap ;
+           GHC.Base.op_zlzd____ := fun {a : Type} {b : Type} =>
+             Functor__MaybeErr_op_zlzd__ |}.
 
 Local Definition Applicative__MaybeErr_op_zlztzg__ {inst_err}
    : forall {a} {b},
@@ -63,56 +66,66 @@ Local Definition Applicative__MaybeErr_op_zlztzg__ {inst_err}
       | Failed e => Failed e
       end.
 
-Local Definition Applicative__MaybeErr_liftA2 {inst_err}
-   : forall {a} {b} {c},
+Local Definition Applicative__MaybeErr_liftA2 {inst_err : Type}
+   : forall {a : Type},
+     forall {b : Type},
+     forall {c : Type},
      (a -> b -> c) ->
-     (MaybeErr inst_err) a -> (MaybeErr inst_err) b -> (MaybeErr inst_err) c :=
-  fun {a} {b} {c} =>
+     MaybeErr inst_err a -> MaybeErr inst_err b -> MaybeErr inst_err c :=
+  fun {a : Type} {b : Type} {c : Type} =>
     fun f x => Applicative__MaybeErr_op_zlztzg__ (GHC.Base.fmap f x).
 
-Local Definition Applicative__MaybeErr_op_ztzg__ {inst_err}
-   : forall {a} {b},
-     (MaybeErr inst_err) a -> (MaybeErr inst_err) b -> (MaybeErr inst_err) b :=
-  fun {a} {b} =>
+Local Definition Applicative__MaybeErr_op_ztzg__ {inst_err : Type}
+   : forall {a : Type},
+     forall {b : Type},
+     MaybeErr inst_err a -> MaybeErr inst_err b -> MaybeErr inst_err b :=
+  fun {a : Type} {b : Type} =>
     fun a1 a2 => Applicative__MaybeErr_op_zlztzg__ (GHC.Base.id GHC.Base.<$ a1) a2.
 
-Local Definition Applicative__MaybeErr_pure {inst_err}
-   : forall {a}, a -> (MaybeErr inst_err) a :=
-  fun {a} => Succeeded.
+Local Definition Applicative__MaybeErr_pure {inst_err : Type}
+   : forall {a : Type}, a -> MaybeErr inst_err a :=
+  fun {a : Type} => Succeeded.
 
-Program Instance Applicative__MaybeErr {err}
+Program Instance Applicative__MaybeErr {err : Type}
    : GHC.Base.Applicative (MaybeErr err) :=
   fun _ k__ =>
-    k__ {| GHC.Base.liftA2__ := fun {a} {b} {c} => Applicative__MaybeErr_liftA2 ;
-           GHC.Base.op_zlztzg____ := fun {a} {b} => Applicative__MaybeErr_op_zlztzg__ ;
-           GHC.Base.op_ztzg____ := fun {a} {b} => Applicative__MaybeErr_op_ztzg__ ;
-           GHC.Base.pure__ := fun {a} => Applicative__MaybeErr_pure |}.
+    k__ {| GHC.Base.liftA2__ := fun {a : Type} {b : Type} {c : Type} =>
+             Applicative__MaybeErr_liftA2 ;
+           GHC.Base.op_zlztzg____ := fun {a : Type} {b : Type} =>
+             Applicative__MaybeErr_op_zlztzg__ ;
+           GHC.Base.op_ztzg____ := fun {a : Type} {b : Type} =>
+             Applicative__MaybeErr_op_ztzg__ ;
+           GHC.Base.pure__ := fun {a : Type} => Applicative__MaybeErr_pure |}.
 
-Local Definition Monad__MaybeErr_op_zgzgze__ {inst_err}
-   : forall {a} {b},
-     (MaybeErr inst_err) a ->
-     (a -> (MaybeErr inst_err) b) -> (MaybeErr inst_err) b :=
-  fun {a} {b} =>
+Local Definition Monad__MaybeErr_op_zgzgze__ {inst_err : Type}
+   : forall {a : Type},
+     forall {b : Type},
+     MaybeErr inst_err a -> (a -> MaybeErr inst_err b) -> MaybeErr inst_err b :=
+  fun {a : Type} {b : Type} =>
     fun arg_0__ arg_1__ =>
       match arg_0__, arg_1__ with
       | Succeeded v, k => k v
       | Failed e, _ => Failed e
       end.
 
-Local Definition Monad__MaybeErr_op_zgzg__ {inst_err}
-   : forall {a} {b},
-     (MaybeErr inst_err) a -> (MaybeErr inst_err) b -> (MaybeErr inst_err) b :=
-  fun {a} {b} => fun m k => Monad__MaybeErr_op_zgzgze__ m (fun arg_0__ => k).
+Local Definition Monad__MaybeErr_op_zgzg__ {inst_err : Type}
+   : forall {a : Type},
+     forall {b : Type},
+     MaybeErr inst_err a -> MaybeErr inst_err b -> MaybeErr inst_err b :=
+  fun {a : Type} {b : Type} =>
+    fun m k => Monad__MaybeErr_op_zgzgze__ m (fun arg_0__ => k).
 
-Local Definition Monad__MaybeErr_return_ {inst_err}
-   : forall {a}, a -> (MaybeErr inst_err) a :=
-  fun {a} => GHC.Base.pure.
+Local Definition Monad__MaybeErr_return_ {inst_err : Type}
+   : forall {a : Type}, a -> MaybeErr inst_err a :=
+  fun {a : Type} => GHC.Base.pure.
 
-Program Instance Monad__MaybeErr {err} : GHC.Base.Monad (MaybeErr err) :=
+Program Instance Monad__MaybeErr {err : Type} : GHC.Base.Monad (MaybeErr err) :=
   fun _ k__ =>
-    k__ {| GHC.Base.op_zgzg____ := fun {a} {b} => Monad__MaybeErr_op_zgzg__ ;
-           GHC.Base.op_zgzgze____ := fun {a} {b} => Monad__MaybeErr_op_zgzgze__ ;
-           GHC.Base.return___ := fun {a} => Monad__MaybeErr_return_ |}.
+    k__ {| GHC.Base.op_zgzg____ := fun {a : Type} {b : Type} =>
+             Monad__MaybeErr_op_zgzg__ ;
+           GHC.Base.op_zgzgze____ := fun {a : Type} {b : Type} =>
+             Monad__MaybeErr_op_zgzgze__ ;
+           GHC.Base.return___ := fun {a : Type} => Monad__MaybeErr_return_ |}.
 
 (* Skipping definition `Maybes.firstJust' *)
 
@@ -127,7 +140,7 @@ Definition expectJust {a} `{GHC.Err.Default a}
         GHC.Err.error (Coq.Init.Datatypes.app (GHC.Base.hs_string__ "expectJust ") err)
     end.
 
-Definition whenIsJust {m} {a} `{GHC.Base.Monad m}
+Definition whenIsJust {m : Type -> Type} {a : Type} `{GHC.Base.Monad m}
    : option a -> (a -> m unit) -> m unit :=
   fun arg_0__ arg_1__ =>
     match arg_0__, arg_1__ with
@@ -135,23 +148,23 @@ Definition whenIsJust {m} {a} `{GHC.Base.Monad m}
     | None, _ => GHC.Base.return_ tt
     end.
 
-Definition orElse {a} : option a -> a -> a :=
+Definition orElse {a : Type} : option a -> a -> a :=
   GHC.Base.flip Data.Maybe.fromMaybe.
 
-Definition liftMaybeT {m} {a} `{GHC.Base.Monad m}
+Definition liftMaybeT {m : Type -> Type} {a : Type} `{GHC.Base.Monad m}
    : m a -> Control.Monad.Trans.Maybe.MaybeT m a :=
   fun act => Control.Monad.Trans.Maybe.Mk_MaybeT (GHC.Base.liftM Some act).
 
 (* Skipping definition `Maybes.tryMaybeT' *)
 
-Definition isSuccess {err} {val} : MaybeErr err val -> bool :=
+Definition isSuccess {err : Type} {val : Type} : MaybeErr err val -> bool :=
   fun arg_0__ => match arg_0__ with | Succeeded _ => true | Failed _ => false end.
 
-Definition failME {err} {val} : err -> MaybeErr err val :=
+Definition failME {err : Type} {val : Type} : err -> MaybeErr err val :=
   fun e => Failed e.
 
 (* External variables:
-     None Some bool false option true tt unit Control.Monad.Trans.Maybe.MaybeT
+     None Some Type bool false option true tt unit Control.Monad.Trans.Maybe.MaybeT
      Control.Monad.Trans.Maybe.Mk_MaybeT Coq.Init.Datatypes.app Data.Maybe.fromMaybe
      GHC.Base.Applicative GHC.Base.Functor GHC.Base.Monad GHC.Base.String
      GHC.Base.const GHC.Base.flip GHC.Base.fmap GHC.Base.fmap__ GHC.Base.id
