examples/ghc/lib/State.v
@@ -28,96 +28,110 @@ Definition runState' {s} {a} (arg_0__ : State s a) :=
 
 (* Converted value declarations: *)
 
-Local Definition Functor__State_fmap {inst_s}
-   : forall {a} {b}, (a -> b) -> (State inst_s) a -> (State inst_s) b :=
-  fun {a} {b} =>
+Local Definition Functor__State_fmap {inst_s : Type}
+   : forall {a : Type},
+     forall {b : Type}, (a -> b) -> State inst_s a -> State inst_s b :=
+  fun {a : Type} {b : Type} =>
     fun f m => Mk_State (fun s => let 'pair r s' := runState' m s in pair (f r) s').
 
-Local Definition Functor__State_op_zlzd__ {inst_s}
-   : forall {a} {b}, a -> (State inst_s) b -> (State inst_s) a :=
-  fun {a} {b} => Functor__State_fmap GHC.Base.∘ GHC.Base.const.
+Local Definition Functor__State_op_zlzd__ {inst_s : Type}
+   : forall {a : Type},
+     forall {b : Type}, a -> State inst_s b -> State inst_s a :=
+  fun {a : Type} {b : Type} => Functor__State_fmap GHC.Base.∘ GHC.Base.const.
 
-Program Instance Functor__State {s} : GHC.Base.Functor (State s) :=
+Program Instance Functor__State {s : Type} : GHC.Base.Functor (State s) :=
   fun _ k__ =>
-    k__ {| GHC.Base.fmap__ := fun {a} {b} => Functor__State_fmap ;
-           GHC.Base.op_zlzd____ := fun {a} {b} => Functor__State_op_zlzd__ |}.
+    k__ {| GHC.Base.fmap__ := fun {a : Type} {b : Type} => Functor__State_fmap ;
+           GHC.Base.op_zlzd____ := fun {a : Type} {b : Type} =>
+             Functor__State_op_zlzd__ |}.
 
-Local Definition Applicative__State_op_zlztzg__ {inst_s}
-   : forall {a} {b},
-     (State inst_s) (a -> b) -> (State inst_s) a -> (State inst_s) b :=
-  fun {a} {b} =>
+Local Definition Applicative__State_op_zlztzg__ {inst_s : Type}
+   : forall {a : Type},
+     forall {b : Type}, State inst_s (a -> b) -> State inst_s a -> State inst_s b :=
+  fun {a : Type} {b : Type} =>
     fun m n =>
       Mk_State (fun s =>
                   let 'pair f s' := runState' m s in
                   let 'pair x s'' := runState' n s' in
                   pair (f x) s'').
 
-Local Definition Applicative__State_liftA2 {inst_s}
-   : forall {a} {b} {c},
-     (a -> b -> c) -> (State inst_s) a -> (State inst_s) b -> (State inst_s) c :=
-  fun {a} {b} {c} =>
+Local Definition Applicative__State_liftA2 {inst_s : Type}
+   : forall {a : Type},
+     forall {b : Type},
+     forall {c : Type},
+     (a -> b -> c) -> State inst_s a -> State inst_s b -> State inst_s c :=
+  fun {a : Type} {b : Type} {c : Type} =>
     fun f x => Applicative__State_op_zlztzg__ (GHC.Base.fmap f x).
 
-Local Definition Applicative__State_op_ztzg__ {inst_s}
-   : forall {a} {b}, (State inst_s) a -> (State inst_s) b -> (State inst_s) b :=
-  fun {a} {b} =>
+Local Definition Applicative__State_op_ztzg__ {inst_s : Type}
+   : forall {a : Type},
+     forall {b : Type}, State inst_s a -> State inst_s b -> State inst_s b :=
+  fun {a : Type} {b : Type} =>
     fun a1 a2 => Applicative__State_op_zlztzg__ (GHC.Base.id GHC.Base.<$ a1) a2.
 
-Local Definition Applicative__State_pure {inst_s}
-   : forall {a}, a -> (State inst_s) a :=
-  fun {a} => fun x => Mk_State (fun s => pair x s).
+Local Definition Applicative__State_pure {inst_s : Type}
+   : forall {a : Type}, a -> State inst_s a :=
+  fun {a : Type} => fun x => Mk_State (fun s => pair x s).
 
-Program Instance Applicative__State {s} : GHC.Base.Applicative (State s) :=
+Program Instance Applicative__State {s : Type}
+   : GHC.Base.Applicative (State s) :=
   fun _ k__ =>
-    k__ {| GHC.Base.liftA2__ := fun {a} {b} {c} => Applicative__State_liftA2 ;
-           GHC.Base.op_zlztzg____ := fun {a} {b} => Applicative__State_op_zlztzg__ ;
-           GHC.Base.op_ztzg____ := fun {a} {b} => Applicative__State_op_ztzg__ ;
-           GHC.Base.pure__ := fun {a} => Applicative__State_pure |}.
+    k__ {| GHC.Base.liftA2__ := fun {a : Type} {b : Type} {c : Type} =>
+             Applicative__State_liftA2 ;
+           GHC.Base.op_zlztzg____ := fun {a : Type} {b : Type} =>
+             Applicative__State_op_zlztzg__ ;
+           GHC.Base.op_ztzg____ := fun {a : Type} {b : Type} =>
+             Applicative__State_op_ztzg__ ;
+           GHC.Base.pure__ := fun {a : Type} => Applicative__State_pure |}.
 
-Local Definition Monad__State_op_zgzgze__ {inst_s}
-   : forall {a} {b},
-     (State inst_s) a -> (a -> (State inst_s) b) -> (State inst_s) b :=
-  fun {a} {b} =>
+Local Definition Monad__State_op_zgzgze__ {inst_s : Type}
+   : forall {a : Type},
+     forall {b : Type}, State inst_s a -> (a -> State inst_s b) -> State inst_s b :=
+  fun {a : Type} {b : Type} =>
     fun m n =>
       Mk_State (fun s => let 'pair r s' := runState' m s in runState' (n r) s').
 
-Local Definition Monad__State_op_zgzg__ {inst_s}
-   : forall {a} {b}, (State inst_s) a -> (State inst_s) b -> (State inst_s) b :=
-  fun {a} {b} => fun m k => Monad__State_op_zgzgze__ m (fun arg_0__ => k).
+Local Definition Monad__State_op_zgzg__ {inst_s : Type}
+   : forall {a : Type},
+     forall {b : Type}, State inst_s a -> State inst_s b -> State inst_s b :=
+  fun {a : Type} {b : Type} =>
+    fun m k => Monad__State_op_zgzgze__ m (fun arg_0__ => k).
 
-Local Definition Monad__State_return_ {inst_s}
-   : forall {a}, a -> (State inst_s) a :=
-  fun {a} => GHC.Base.pure.
+Local Definition Monad__State_return_ {inst_s : Type}
+   : forall {a : Type}, a -> State inst_s a :=
+  fun {a : Type} => GHC.Base.pure.
 
-Program Instance Monad__State {s} : GHC.Base.Monad (State s) :=
+Program Instance Monad__State {s : Type} : GHC.Base.Monad (State s) :=
   fun _ k__ =>
-    k__ {| GHC.Base.op_zgzg____ := fun {a} {b} => Monad__State_op_zgzg__ ;
-           GHC.Base.op_zgzgze____ := fun {a} {b} => Monad__State_op_zgzgze__ ;
-           GHC.Base.return___ := fun {a} => Monad__State_return_ |}.
+    k__ {| GHC.Base.op_zgzg____ := fun {a : Type} {b : Type} =>
+             Monad__State_op_zgzg__ ;
+           GHC.Base.op_zgzgze____ := fun {a : Type} {b : Type} =>
+             Monad__State_op_zgzgze__ ;
+           GHC.Base.return___ := fun {a : Type} => Monad__State_return_ |}.
 
-Definition get {s} : State s s :=
+Definition get {s : Type} : State s s :=
   Mk_State (fun s => pair s s).
 
-Definition gets {s} {a} : (s -> a) -> State s a :=
+Definition gets {s : Type} {a : Type} : (s -> a) -> State s a :=
   fun f => Mk_State (fun s => pair (f s) s).
 
-Definition put {s} : s -> State s unit :=
+Definition put {s : Type} : s -> State s unit :=
   fun s' => Mk_State (fun arg_0__ => pair tt s').
 
-Definition modify {s} : (s -> s) -> State s unit :=
+Definition modify {s : Type} : (s -> s) -> State s unit :=
   fun f => Mk_State (fun s => pair tt (f s)).
 
-Definition evalState {s} {a} : State s a -> s -> a :=
+Definition evalState {s : Type} {a : Type} : State s a -> s -> a :=
   fun s i => let 'pair a _ := runState' s i in a.
 
-Definition execState {s} {a} : State s a -> s -> s :=
+Definition execState {s : Type} {a : Type} : State s a -> s -> s :=
   fun s i => let 'pair _ s' := runState' s i in s'.
 
-Definition runState {s} {a} : State s a -> s -> (a * s)%type :=
+Definition runState {s : Type} {a : Type} : State s a -> s -> (a * s)%type :=
   fun s i => let 'pair a s' := runState' s i in pair a s'.
 
 (* External variables:
-     op_zt__ pair tt unit GHC.Base.Applicative GHC.Base.Functor GHC.Base.Monad
+     Type op_zt__ pair tt unit GHC.Base.Applicative GHC.Base.Functor GHC.Base.Monad
      GHC.Base.const GHC.Base.fmap GHC.Base.fmap__ GHC.Base.id GHC.Base.liftA2__
      GHC.Base.op_z2218U__ GHC.Base.op_zgzg____ GHC.Base.op_zgzgze____
      GHC.Base.op_zlzd__ GHC.Base.op_zlzd____ GHC.Base.op_zlztzg____
