examples/ghc/lib/FastStringEnv.v
@@ -25,71 +25,75 @@ Definition DFastStringEnv :=
 
 (* Converted value declarations: *)
 
-Axiom emptyFsEnv : forall {a}, FastStringEnv a.
+Axiom emptyFsEnv : forall {a : Type}, FastStringEnv a.
 
-Axiom unitFsEnv : forall {a}, FastString.FastString -> a -> FastStringEnv a.
+Axiom unitFsEnv : forall {a : Type},
+                  FastString.FastString -> a -> FastStringEnv a.
 
-Axiom extendFsEnv : forall {a},
+Axiom extendFsEnv : forall {a : Type},
                     FastStringEnv a -> FastString.FastString -> a -> FastStringEnv a.
 
-Axiom extendFsEnvList : forall {a},
+Axiom extendFsEnvList : forall {a : Type},
                         FastStringEnv a -> list (FastString.FastString * a)%type -> FastStringEnv a.
 
-Axiom lookupFsEnv : forall {a},
+Axiom lookupFsEnv : forall {a : Type},
                     FastStringEnv a -> FastString.FastString -> option a.
 
-Axiom alterFsEnv : forall {a},
+Axiom alterFsEnv : forall {a : Type},
                    (option a -> option a) ->
                    FastStringEnv a -> FastString.FastString -> FastStringEnv a.
 
-Axiom mkFsEnv : forall {a},
+Axiom mkFsEnv : forall {a : Type},
                 list (FastString.FastString * a)%type -> FastStringEnv a.
 
-Axiom elemFsEnv : forall {a}, FastString.FastString -> FastStringEnv a -> bool.
+Axiom elemFsEnv : forall {a : Type},
+                  FastString.FastString -> FastStringEnv a -> bool.
 
-Axiom plusFsEnv : forall {a},
+Axiom plusFsEnv : forall {a : Type},
                   FastStringEnv a -> FastStringEnv a -> FastStringEnv a.
 
-Axiom plusFsEnv_C : forall {a},
+Axiom plusFsEnv_C : forall {a : Type},
                     (a -> a -> a) -> FastStringEnv a -> FastStringEnv a -> FastStringEnv a.
 
-Axiom extendFsEnv_C : forall {a},
+Axiom extendFsEnv_C : forall {a : Type},
                       (a -> a -> a) ->
                       FastStringEnv a -> FastString.FastString -> a -> FastStringEnv a.
 
-Axiom mapFsEnv : forall {elt1} {elt2},
+Axiom mapFsEnv : forall {elt1 : Type},
+                 forall {elt2 : Type},
                  (elt1 -> elt2) -> FastStringEnv elt1 -> FastStringEnv elt2.
 
-Axiom extendFsEnv_Acc : forall {a} {b},
+Axiom extendFsEnv_Acc : forall {a : Type},
+                        forall {b : Type},
                         (a -> b -> b) ->
                         (a -> b) -> FastStringEnv b -> FastString.FastString -> a -> FastStringEnv b.
 
-Axiom extendFsEnvList_C : forall {a},
+Axiom extendFsEnvList_C : forall {a : Type},
                           (a -> a -> a) ->
                           FastStringEnv a -> list (FastString.FastString * a)%type -> FastStringEnv a.
 
-Axiom delFromFsEnv : forall {a},
+Axiom delFromFsEnv : forall {a : Type},
                      FastStringEnv a -> FastString.FastString -> FastStringEnv a.
 
-Axiom delListFromFsEnv : forall {a},
+Axiom delListFromFsEnv : forall {a : Type},
                          FastStringEnv a -> list FastString.FastString -> FastStringEnv a.
 
-Axiom filterFsEnv : forall {elt},
+Axiom filterFsEnv : forall {elt : Type},
                     (elt -> bool) -> FastStringEnv elt -> FastStringEnv elt.
 
-Axiom lookupFsEnv_NF : forall {a},
+Axiom lookupFsEnv_NF : forall {a : Type},
                        FastStringEnv a -> FastString.FastString -> a.
 
-Axiom emptyDFsEnv : forall {a}, DFastStringEnv a.
+Axiom emptyDFsEnv : forall {a : Type}, DFastStringEnv a.
 
-Axiom dFsEnvElts : forall {a}, DFastStringEnv a -> list a.
+Axiom dFsEnvElts : forall {a : Type}, DFastStringEnv a -> list a.
 
-Axiom mkDFsEnv : forall {a},
+Axiom mkDFsEnv : forall {a : Type},
                  list (FastString.FastString * a)%type -> DFastStringEnv a.
 
-Axiom lookupDFsEnv : forall {a},
+Axiom lookupDFsEnv : forall {a : Type},
                      DFastStringEnv a -> FastString.FastString -> option a.
 
 (* External variables:
-     bool list op_zt__ option FastString.FastString UniqFM.UniqFM
+     Type bool list op_zt__ option FastString.FastString UniqFM.UniqFM
 *)
